@prefix : <https://w3id.org/moneygraph/ns/ontology/> .
@prefix mg: <https://w3id.org/moneygraph/ns/ontology/> .
@prefix mgx: <https://w3id.org/moneygraph/ns/taxonomy/> .
@prefix owl: <http://www.w3.org/2002/07/owl#> .
@prefix rdf: <http://www.w3.org/1999/02/22-rdf-syntax-ns#> .
@prefix xml: <http://www.w3.org/XML/1998/namespace> .
@prefix xsd: <http://www.w3.org/2001/XMLSchema#> .
@prefix gist: <https://w3id.org/semanticarts/ns/ontology/gist/> .
@prefix rdfs: <http://www.w3.org/2000/01/rdf-schema#> .
@base <https://w3id.org/moneygraph/ns/ontology/> .

<https://w3id.org/moneygraph/o/ontology/> rdf:type owl:Ontology ;
                                           owl:versionIRI <https://w3id.org/moneygraph/o/moneygraph_1.0.0> ;
                                           owl:imports <https://w3id.org/semanticarts/ontology/gistCore12.0.1> ,
                                                       <https://w3id.org/semanticarts/ontology/gistDCAcct1.0.0> ;
                                           rdfs:comment """Moneygraph is a semantic data model for a personal investment portfolio supporting stocks, bonds, exchange-traded funds (ETFs), and mutual funds. The model includes a formal ontology of concepts (i.e. classes) and their relations, a taxonomy of controlled vocabulary terms (instances), and a set of scripts that enable loading and transforming data into a graph that conforms to the model.
The Moneygraph ontology is based on gist, a minimalist upper ontology maintained by Semantic Arts Inc.""" .

#################################################################
#    Annotation properties
#################################################################

###  http://www.w3.org/2004/02/skos/core#editorialNote
<http://www.w3.org/2004/02/skos/core#editorialNote> rdf:type owl:AnnotationProperty .


###  https://w3id.org/moneygraph/ns/ontology/lastUpdated
mg:lastUpdated rdf:type owl:AnnotationProperty ;
               rdfs:subPropertyOf <http://www.w3.org/2004/02/skos/core#scopeNote> .


###  https://w3id.org/semanticarts/ns/ontology/gist/conversionFactor
gist:conversionFactor rdf:type owl:AnnotationProperty .


###  https://w3id.org/semanticarts/ns/ontology/gist/hasBaseUnit
gist:hasBaseUnit rdf:type owl:AnnotationProperty .


###  https://w3id.org/semanticarts/ns/ontology/gist/hasDenominator
gist:hasDenominator rdf:type owl:AnnotationProperty .


###  https://w3id.org/semanticarts/ns/ontology/gist/hasNumerator
gist:hasNumerator rdf:type owl:AnnotationProperty .


###  https://w3id.org/semanticarts/ns/ontology/gist/unitSymbol
gist:unitSymbol rdf:type owl:AnnotationProperty .


#################################################################
#    Datatypes
#################################################################

###  https://w3id.org/semanticarts/ns/ontology/fhir/aminoAcidSequence
<https://w3id.org/semanticarts/ns/ontology/fhir/aminoAcidSequence> rdf:type rdfs:Datatype ;
                                                                   <http://www.w3.org/2004/02/skos/core#prefLabel> "aminoAcidSequence" .


#################################################################
#    Object Properties
#################################################################

###  https://w3id.org/moneygraph/ns/ontology/hasInterestPaymentTerms
mg:hasInterestPaymentTerms rdf:type owl:ObjectProperty ;
                           rdfs:subPropertyOf gist:conformsTo ;
                           rdfs:seeAlso "https://spec.edmcouncil.org/fibo/ontology/SEC/Debt/DebtInstruments/hasInterestPaymentTerms" ;
                           <http://www.w3.org/2004/02/skos/core#prefLabel> "has interest payment terms" .


###  https://w3id.org/moneygraph/ns/ontology/hasRepaymentTerms
mg:hasRepaymentTerms rdf:type owl:ObjectProperty ;
                     rdfs:subPropertyOf gist:conformsTo ;
                     rdfs:seeAlso "fibo-sec-dbt-dbti:hasRepaymentTerms"^^xsd:anyURI ;
                     <http://www.w3.org/2004/02/skos/core#definition> "Relates the subject to a specification of loan repayment conditions." ;
                     <http://www.w3.org/2004/02/skos/core#prefLabel> "has repayment terms" .


###  https://w3id.org/moneygraph/ns/ontology/isIssuedBy
mg:isIssuedBy rdf:type owl:ObjectProperty ;
              rdfs:subPropertyOf gist:isAllocatedBy ;
              rdfs:range gist:Organization ;
              <http://www.w3.org/2004/02/skos/core#definition> "Relates to the organization that issued a security or financial instrument, e.g. common stock or a bond." ;
              <http://www.w3.org/2004/02/skos/core#prefLabel> "is issued by" .


###  https://w3id.org/moneygraph/ns/taxonomy/hasInterestRate
mgx:hasInterestRate rdf:type owl:ObjectProperty ;
                    rdfs:subPropertyOf gist:hasMagnitude ;
                    rdfs:seeAlso "https://spec.edmcouncil.org/fibo/ontology/FBC/DebtAndEquities/Debt/hasInterestRate" ;
                    <http://www.w3.org/2004/02/skos/core#prefLabel> "has interest rate" .


#################################################################
#    Data properties
#################################################################

###  https://w3id.org/moneygraph/ns/ontology/assessmentDate
mg:assessmentDate rdf:type owl:DatatypeProperty ;
                  rdfs:subPropertyOf gist:endDate ;
                  rdfs:isDefinedBy <https://w3id.org/moneygraph/o/ontology/> ;
                  <http://www.w3.org/2004/02/skos/core#definition> "Date on which the value of an investment is reported or assessed." ;
                  <http://www.w3.org/2004/02/skos/core#prefLabel> "assessment date" .


###  https://w3id.org/moneygraph/ns/ontology/callable
mg:callable rdf:type owl:DatatypeProperty ;
            rdfs:domain mg:Bond ;
            rdfs:range xsd:boolean ;
            <http://www.w3.org/2004/02/skos/core#definition> "True if the subject (typically a bond) may be redeemed before its maturity date." ;
            <http://www.w3.org/2004/02/skos/core#prefLabel> "callable" .


###  https://w3id.org/moneygraph/ns/ontology/longDescription
mg:longDescription rdf:type owl:DatatypeProperty ;
                   rdfs:subPropertyOf gist:description ;
                   <http://www.w3.org/2004/02/skos/core#definition> "When there is more to say..." ;
                   <http://www.w3.org/2004/02/skos/core#prefLabel> "longDescription" .


###  https://w3id.org/moneygraph/ns/ontology/plannedOccursDate
mg:plannedOccursDate rdf:type owl:DatatypeProperty ;
                     rdfs:subPropertyOf gist:atDate ;
                     <http://www.w3.org/2004/02/skos/core#definition> "The date on which something is planned or expected to occur." ;
                     <http://www.w3.org/2004/02/skos/core#prefLabel> "planned occurs date" .


###  https://w3id.org/semanticarts/ns/ontology/gist/atDate
gist:atDate rdf:type owl:DatatypeProperty .


#################################################################
#    Classes
#################################################################

###  https://w3id.org/moneygraph/ns/ontology/Bond
mg:Bond rdf:type owl:Class ;
        owl:equivalentClass [ owl:intersectionOf ( gist:FinancialInstrument
                                                   [ rdf:type owl:Restriction ;
                                                     owl:onProperty mg:hasInterestPaymentTerms ;
                                                     owl:someValuesFrom mg:CouponPaymentTerms
                                                   ]
                                                   [ rdf:type owl:Restriction ;
                                                     owl:onProperty gist:isCategorizedBy ;
                                                     owl:hasValue mgx:_MarketableSecurityType_bond
                                                   ]
                                                 ) ;
                              rdf:type owl:Class
                            ] ;
        <http://www.w3.org/2004/02/skos/core#definition> "A portion of a debt on which the owner receives interest periodically before being repaid the initial loan amount." ;
        <http://www.w3.org/2004/02/skos/core#prefLabel> "Bond" .


###  https://w3id.org/moneygraph/ns/ontology/BondCoupon
mg:BondCoupon rdf:type owl:Class ;
              rdfs:subClassOf gist:Percentage ,
                              [ owl:intersectionOf ( gist:Percentage
                                                     [ rdf:type owl:Restriction ;
                                                       owl:onProperty gist:hasUnitOfMeasure ;
                                                       owl:hasValue mg:_RatioUnit_annualInterestRate
                                                     ]
                                                     [ rdf:type owl:Restriction ;
                                                       owl:onProperty gist:isCategorizedBy ;
                                                       owl:hasValue mgx:_Aspect_annualInterestRate
                                                     ]
                                                   ) ;
                                rdf:type owl:Class
                              ] ;
              rdfs:seeAlso "https://spec.edmcouncil.org/fibo/ontology/SEC/Debt/Bonds/BondCoupon" ,
                           "https://www.investopedia.com/terms/c/coupon.asp" ;
              <http://www.w3.org/2004/02/skos/core#definition> "The annual interest rate on a debt instrument making periodic interest payments to the instrument holder." ;
              <http://www.w3.org/2004/02/skos/core#prefLabel> "Bond Coupon" .


###  https://w3id.org/moneygraph/ns/ontology/BondRating
mg:BondRating rdf:type owl:Class ;
              rdfs:subClassOf gist:Category ;
              <http://www.w3.org/2004/02/skos/core#definition> "A qualitative assessment of the financial risks associated to a bond, primarily based on the credit worthiness of its issuer. Ratings are provided by specialized agencies such as Dun and Bradstreet." ;
              <http://www.w3.org/2004/02/skos/core#prefLabel> "Bond Rating" .


###  https://w3id.org/moneygraph/ns/ontology/BondRepaymentTerms
mg:BondRepaymentTerms rdf:type owl:Class ;
                      rdfs:subClassOf gist:ContractTerm ;
                      <http://www.w3.org/2004/02/skos/core#definition> "A specification of the bond maturity and principal repayment event. Typically includes bond principal amount and maturity date." ;
                      <http://www.w3.org/2004/02/skos/core#prefLabel> "Bond Repayment Terms" .


###  https://w3id.org/moneygraph/ns/ontology/CashAccount
mg:CashAccount rdf:type owl:Class ;
               rdfs:subClassOf gist:AssetsHeldAwayAccount ;
               owl:disjointWith gist:InvestmentAccount ;
               <http://www.w3.org/2004/02/skos/core#definition> "Represents the cash balances, in different currencies, held by a third party on behalf of the owner." ;
               <http://www.w3.org/2004/02/skos/core#prefLabel> "CashAccount" .


###  https://w3id.org/moneygraph/ns/ontology/CommonStock
mg:CommonStock rdf:type owl:Class ;
               owl:equivalentClass [ owl:intersectionOf ( mg:MarketableSecurity
                                                          [ rdf:type owl:Restriction ;
                                                            owl:onProperty gist:isCategorizedBy ;
                                                            owl:hasValue mgx:_MarketableSecurityType_common_stock
                                                          ]
                                                        ) ;
                                     rdf:type owl:Class
                                   ] ;
               rdfs:subClassOf mg:MarketableSecurity ;
               <http://www.w3.org/2004/02/skos/core#definition> "A general class of securities conferring partial ownership of a corporation to the shareholder." ;
               <http://www.w3.org/2004/02/skos/core#prefLabel> "Common Stock" .


###  https://w3id.org/moneygraph/ns/ontology/CouponPayment
mg:CouponPayment rdf:type owl:Class ;
                 owl:equivalentClass [ owl:intersectionOf ( gist:Event
                                                            [ rdf:type owl:Restriction ;
                                                              owl:onProperty gist:isCategorizedBy ;
                                                              owl:hasValue mgx:_FinancialBusinessEventType_interestRemittance
                                                            ]
                                                          ) ;
                                       rdf:type owl:Class
                                     ] ;
                 rdfs:subClassOf gist:RemittanceEvent ;
                 rdfs:seeAlso "fibo-sec-dbt-bnd:CouponPayment"^^xsd:anyURI ;
                 <http://www.w3.org/2004/02/skos/core#definition> "Receipt of a bond interest payment, usually on a fixed schedule." ;
                 <http://www.w3.org/2004/02/skos/core#prefLabel> "Coupon Payment" .


###  https://w3id.org/moneygraph/ns/ontology/CouponPaymentSchedule
mg:CouponPaymentSchedule rdf:type owl:Class ;
                         owl:equivalentClass [ rdf:type owl:Restriction ;
                                               owl:onProperty gist:hasMember ;
                                               owl:someValuesFrom mg:CouponPayment
                                             ] ;
                         rdfs:subClassOf gist:Collection ;
                         <http://www.w3.org/2004/02/skos/core#definition> "A series of payments of bond coupons, either planned or past." .


###  https://w3id.org/moneygraph/ns/ontology/CouponPaymentTerms
mg:CouponPaymentTerms rdf:type owl:Class ;
                      rdfs:subClassOf gist:ContractTerm ;
                      rdfs:seeAlso "https://spec.edmcouncil.org/fibo/ontology/SEC/Debt/Bonds/CouponPaymentTerms"^^xsd:anyURI ;
                      <http://www.w3.org/2004/02/skos/core#prefLabel> "Coupon Payment Terms" .


###  https://w3id.org/moneygraph/ns/ontology/ExchangeTradedFund
mg:ExchangeTradedFund rdf:type owl:Class ;
                      owl:equivalentClass [ owl:intersectionOf ( mg:MarketableSecurity
                                                                 [ rdf:type owl:Restriction ;
                                                                   owl:onProperty gist:isCategorizedBy ;
                                                                   owl:hasValue mgx:_MarketableSecurityType_exchange_traded_fund
                                                                 ]
                                                               ) ;
                                            rdf:type owl:Class
                                          ] ;
                      rdfs:subClassOf mg:MarketableSecurity ;
                      <http://www.w3.org/2004/02/skos/core#definition> "A basket security whose value is adjusted continously to track that of a larger index of stocks but which, unlike mutual funds, is traded on a public exchange." .


###  https://w3id.org/moneygraph/ns/ontology/FixedInterestRate
mg:FixedInterestRate rdf:type owl:Class ;
                     rdfs:subClassOf gist:Percentage ,
                                     gist:ReferenceValue ;
                     <http://www.w3.org/2004/02/skos/core#prefLabel> "Fixed Interest Rate" .


###  https://w3id.org/moneygraph/ns/ontology/InvestmentPortfolio
mg:InvestmentPortfolio rdf:type owl:Class ;
                       owl:equivalentClass [ owl:intersectionOf ( gist:Collection
                                                                  [ rdf:type owl:Restriction ;
                                                                    owl:onProperty gist:hasMember ;
                                                                    owl:someValuesFrom gist:FinancialAccount
                                                                  ]
                                                                ) ;
                                             rdf:type owl:Class
                                           ] ;
                       rdfs:subClassOf gist:Collection ;
                       <http://www.w3.org/2004/02/skos/core#definition> "A collection of investment accounts that each track an investment asset." ;
                       <http://www.w3.org/2004/02/skos/core#prefLabel> "Investment Portfolio" .


###  https://w3id.org/moneygraph/ns/ontology/MarketableSecurity
mg:MarketableSecurity rdf:type owl:Class ;
                      owl:equivalentClass [ owl:intersectionOf ( gist:FinancialInstrument
                                                                 [ rdf:type owl:Restriction ;
                                                                   owl:onProperty gist:isCategorizedBy ;
                                                                   owl:someValuesFrom mg:MarketableSecurityType
                                                                 ]
                                                                 [ rdf:type owl:Restriction ;
                                                                   owl:onProperty gist:isIdentifiedBy ;
                                                                   owl:someValuesFrom mg:MarketableSecurityIdentifierType
                                                                 ]
                                                               ) ;
                                            rdf:type owl:Class
                                          ] ;
                      rdfs:subClassOf gist:FinancialInstrument ;
                      <http://www.w3.org/2004/02/skos/core#definition> "An instrument of debt or equity, or options to buy and sell, that may be sold on a market." ;
                      <http://www.w3.org/2004/02/skos/core#prefLabel> "Marketable Security" .


###  https://w3id.org/moneygraph/ns/ontology/MarketableSecurityIdentifier
mg:MarketableSecurityIdentifier rdf:type owl:Class ;
                                owl:equivalentClass [ owl:intersectionOf ( gist:ID
                                                                           [ rdf:type owl:Restriction ;
                                                                             owl:onProperty gist:isCategorizedBy ;
                                                                             owl:someValuesFrom mg:MarketableSecurityIdentifierType
                                                                           ]
                                                                         ) ;
                                                      rdf:type owl:Class
                                                    ] ;
                                <http://www.w3.org/2004/02/skos/core#definition> "An identifier for marketable securities, e.g. CUSIP" ;
                                <http://www.w3.org/2004/02/skos/core#prefLabel> "Marketable Security Identifier" .


###  https://w3id.org/moneygraph/ns/ontology/MarketableSecurityIdentifierType
mg:MarketableSecurityIdentifierType rdf:type owl:Class ;
                                    rdfs:subClassOf gist:Category ;
                                    <http://www.w3.org/2004/02/skos/core#definition> "Kinds of IDs used in financial markets, e.g. CUSIP for bonds, exchange symbol for stocks, etc." ;
                                    <http://www.w3.org/2004/02/skos/core#prefLabel> "Marketable Security Identifier Type" .


###  https://w3id.org/moneygraph/ns/ontology/MarketableSecurityType
mg:MarketableSecurityType rdf:type owl:Class ;
                          rdfs:subClassOf gist:Behavior ;
                          <http://www.w3.org/2004/02/skos/core#definition> "Kinds of securities include stocks, bonds, etf." ;
                          <http://www.w3.org/2004/02/skos/core#editorialNote> "Cash is a represented as an instance of Financial Instrument, not Marketable Security, as cash is not \"marketable\" per se." ;
                          <http://www.w3.org/2004/02/skos/core#prefLabel> "Financial Instrument Type" .


###  https://w3id.org/semanticarts/ns/ontology/gist/CurrencyPerDurationUnit
gist:CurrencyPerDurationUnit rdf:type owl:Class .


###  https://w3id.org/semanticarts/ns/ontology/gist/FinancialBusinessEventType
gist:FinancialBusinessEventType rdf:type owl:Class .


###  https://w3id.org/semanticarts/ns/ontology/gist/FinancialInstrument
gist:FinancialInstrument rdf:type owl:Class ;
                         <http://www.w3.org/2004/02/skos/core#prefLabel> "Financial Instrument" .


###  https://w3id.org/semanticarts/ns/ontology/gist/Percentage
gist:Percentage rdf:type owl:Class .


###  https://w3id.org/semanticarts/ns/ontology/gist/RemittanceEvent
gist:RemittanceEvent rdf:type owl:Class .


#################################################################
#    Individuals
#################################################################

###  https://w3id.org/moneygraph/ns/ontology/_365_day_year
mg:_365_day_year rdf:type owl:NamedIndividual ,
                          gist:DurationUnit ;
                 gist:hasBaseUnit gist:_day ;
                 <http://www.w3.org/2004/02/skos/core#definition> "One year defined as exactly 365 24-hour days (not 365.25)." ;
                 <http://www.w3.org/2004/02/skos/core#prefLabel> "365-day year" ;
                 gist:conversionFactor 365 ;
                 gist:unitSymbol "yr" .


###  https://w3id.org/moneygraph/ns/ontology/_CurrencyPerDurationUnit_CADPerDay
mg:_CurrencyPerDurationUnit_CADPerDay rdf:type owl:NamedIndividual ,
                                               gist:CurrencyPerDurationUnit ;
                                      gist:hasDenominator gist:_one_day ;
                                      gist:hasNumerator mgx:_CADollar ;
                                      <http://www.w3.org/2004/02/skos/core#definition> "e.g. number of dollars per day, as in the principal amount of a loan divided by the number of days in its term, from loan issuance to due date." .


###  https://w3id.org/moneygraph/ns/ontology/_CurrencyPerDurationUnit_CADPerYear
mg:_CurrencyPerDurationUnit_CADPerYear rdf:type owl:NamedIndividual ,
                                                gist:CurrencyPerDurationUnit ;
                                       gist:hasDenominator mg:_365_day_year ;
                                       gist:hasNumerator mgx:_CADollar ;
                                       <http://www.w3.org/2004/02/skos/core#definition> "e.g. number of dollars per day, as in the principal amount of a loan divided by the number of days in its term, from loan issuance to due date." .


###  https://w3id.org/moneygraph/ns/ontology/_RatioUnit_annualInterestRate
mg:_RatioUnit_annualInterestRate rdf:type owl:NamedIndividual ,
                                          gist:RatioUnit ;
                                 gist:hasDenominator mg:_CurrencyPerDurationUnit_CADPerYear ;
                                 gist:hasNumerator mg:_CurrencyPerDurationUnit_CADPerYear ;
                                 <http://www.w3.org/2004/02/skos/core#definition> """interest rate = 1 - (principal amount + interest amount for the time period) / principal amount)

interest amount for one period = interest rate for one period * principal amount""" .


###  https://w3id.org/moneygraph/ns/ontology/_RatioUnit_dailyInterestRate
mg:_RatioUnit_dailyInterestRate rdf:type owl:NamedIndividual ,
                                         gist:RatioUnit ;
                                gist:hasDenominator mg:_CurrencyPerDurationUnit_CADPerDay ;
                                gist:hasNumerator mg:_CurrencyPerDurationUnit_CADPerDay ;
                                <http://www.w3.org/2004/02/skos/core#definition> """interest rate = 1 - (principal amount + interest amount for the time period) / principal amount)

interest amount for one period = interest rate for one period * principal amount""" .


###  https://w3id.org/moneygraph/ns/ontology/_RatioUnit_monetaryPerMonetary
mg:_RatioUnit_monetaryPerMonetary rdf:type owl:NamedIndividual ,
                                           gist:CoherentRatioUnit ;
                                  gist:hasDenominator gist:_USDollar ;
                                  gist:hasNumerator gist:_USDollar ;
                                  <http://www.w3.org/2004/02/skos/core#definition> "Amount of money per amount of money, as a percentage." ;
                                  gist:conversionFactor 0.01 .


###  https://w3id.org/moneygraph/ns/ontology/_RatioUnit_totalInvestmentReturnRate
mg:_RatioUnit_totalInvestmentReturnRate rdf:type owl:NamedIndividual ,
                                                 gist:RatioUnit ;
                                        <http://www.w3.org/2004/02/skos/core#definition> "Percentage return on an investment from purchase to today." ;
                                        <http://www.w3.org/2004/02/skos/core#prefLabel> "total investment return rate" .


###  https://w3id.org/moneygraph/ns/taxonomy/_Aspect_annualInterestRate
mgx:_Aspect_annualInterestRate rdf:type owl:NamedIndividual ,
                                        gist:Aspect ;
                               rdfs:isDefinedBy <https://w3id.org/moneygraph/o/ontology/> ;
                               <http://www.w3.org/2004/02/skos/core#definition> "Amount of interest as a percentage value for one year. There is no specific or particular meaning of \"year\" implied here." .


###  https://w3id.org/moneygraph/ns/taxonomy/_Aspect_daysOfInterestPaid
mgx:_Aspect_daysOfInterestPaid rdf:type owl:NamedIndividual ,
                                        gist:Aspect ;
                               <http://www.w3.org/2004/02/skos/core#definition> "At a bond purchase, it is necessary to compensate the previous owner (seller) for the number of days of interest that have accrued since the last coupon payment, but that have not yet been paid." ;
                               <http://www.w3.org/2004/02/skos/core#prefLabel> "days of interest paid" .


###  https://w3id.org/moneygraph/ns/taxonomy/_Aspect_debtInterestAmount
mgx:_Aspect_debtInterestAmount rdf:type owl:NamedIndividual ,
                                        gist:Aspect ;
                               rdfs:isDefinedBy <https://w3id.org/moneygraph/o/ontology/> ;
                               <http://www.w3.org/2004/02/skos/core#definition> "Interest received or paid for a debt (e.g. bond)." .


###  https://w3id.org/moneygraph/ns/taxonomy/_Aspect_debtPrincipalAmount
mgx:_Aspect_debtPrincipalAmount rdf:type owl:NamedIndividual ,
                                         gist:Aspect ;
                                rdfs:isDefinedBy <https://w3id.org/moneygraph/o/ontology/> ;
                                <http://www.w3.org/2004/02/skos/core#definition> "The amount of money representing the principal of a debt, e.g. a bond face value." .


###  https://w3id.org/moneygraph/ns/taxonomy/_Aspect_debtPrincipalRepaymentAmount
mgx:_Aspect_debtPrincipalRepaymentAmount rdf:type owl:NamedIndividual ,
                                                  gist:Aspect ;
                                         rdfs:isDefinedBy <https://w3id.org/moneygraph/o/ontology/> ;
                                         <http://www.w3.org/2004/02/skos/core#definition> "Amount repaid on the principal of a debt." ;
                                         <http://www.w3.org/2004/02/skos/core#prefLabel> "debt principal repayment amount" .


###  https://w3id.org/moneygraph/ns/taxonomy/_Aspect_depositAmount
mgx:_Aspect_depositAmount rdf:type owl:NamedIndividual ,
                                   gist:Aspect ;
                          rdfs:isDefinedBy <https://w3id.org/moneygraph/o/ontology/> ;
                          <http://www.w3.org/2004/02/skos/core#definition> "An amount of money deposited to an account." .


###  https://w3id.org/moneygraph/ns/taxonomy/_Aspect_securityPositionCostAmount
mgx:_Aspect_securityPositionCostAmount rdf:type owl:NamedIndividual ,
                                                gist:Aspect ;
                                       rdfs:isDefinedBy <https://w3id.org/moneygraph/o/ontology/> ;
                                       <http://www.w3.org/2004/02/skos/core#definition> "Price paid for all shares, including fees, of a security." ;
                                       <http://www.w3.org/2004/02/skos/core#prefLabel> "security position cost amount" .


###  https://w3id.org/moneygraph/ns/taxonomy/_Aspect_securityPositionPercentPortfolio
mgx:_Aspect_securityPositionPercentPortfolio rdf:type owl:NamedIndividual ,
                                                      gist:Aspect ;
                                             rdfs:isDefinedBy <https://w3id.org/moneygraph/o/ontology/> ;
                                             <http://www.w3.org/2004/02/skos/core#definition> "The value of a security position as a percentage of the total portfolio's value." .


###  https://w3id.org/moneygraph/ns/taxonomy/_Aspect_securityPositionProfitAmount
mgx:_Aspect_securityPositionProfitAmount rdf:type owl:NamedIndividual ,
                                                  gist:Aspect ;
                                         rdfs:isDefinedBy <https://w3id.org/moneygraph/o/ontology/> ;
                                         <http://www.w3.org/2004/02/skos/core#definition> "Value of the current security position less its initial cost." ;
                                         <http://www.w3.org/2004/02/skos/core#prefLabel> "security position profit amount" .


###  https://w3id.org/moneygraph/ns/taxonomy/_Aspect_securityPositionReturnRatio
mgx:_Aspect_securityPositionReturnRatio rdf:type owl:NamedIndividual ,
                                                 gist:Aspect ;
                                        rdfs:isDefinedBy <https://w3id.org/moneygraph/o/ontology/> ;
                                        <http://www.w3.org/2004/02/skos/core#definition> "Value of an security position divided by its cost." .


###  https://w3id.org/moneygraph/ns/taxonomy/_Aspect_securityPositionValueAmount
mgx:_Aspect_securityPositionValueAmount rdf:type owl:NamedIndividual ,
                                                 gist:Aspect ;
                                        rdfs:isDefinedBy <https://w3id.org/moneygraph/o/ontology/> ;
                                        <http://www.w3.org/2004/02/skos/core#definition> "Assessed value of a position in a security." ;
                                        <http://www.w3.org/2004/02/skos/core#prefLabel> "security position value amount" .


###  https://w3id.org/moneygraph/ns/taxonomy/_Aspect_securityShareAmount
mgx:_Aspect_securityShareAmount rdf:type owl:NamedIndividual ,
                                         gist:Aspect ;
                                rdfs:isDefinedBy <https://w3id.org/moneygraph/o/ontology/> ;
                                <http://www.w3.org/2004/02/skos/core#definition> "The number (may be fractional) of shares in a security, owned, sold, referred to, etc." .


###  https://w3id.org/moneygraph/ns/taxonomy/_Aspect_securityShareDividendAmount
mgx:_Aspect_securityShareDividendAmount rdf:type owl:NamedIndividual ,
                                                 gist:Aspect ;
                                        rdfs:isDefinedBy <https://w3id.org/moneygraph/o/ontology/> ;
                                        <http://www.w3.org/2004/02/skos/core#definition> "Monetary amount of a dividend paid on shares of common stock or an ETF." .


###  https://w3id.org/moneygraph/ns/taxonomy/_Aspect_securityShareUnitPriceAmount
mgx:_Aspect_securityShareUnitPriceAmount rdf:type owl:NamedIndividual ,
                                                  gist:Aspect ;
                                         rdfs:isDefinedBy <https://w3id.org/moneygraph/o/ontology/> ;
                                         <http://www.w3.org/2004/02/skos/core#definition> "Price paid for one share of a security." ;
                                         <http://www.w3.org/2004/02/skos/core#prefLabel> "security share unit price amount" .


###  https://w3id.org/moneygraph/ns/taxonomy/_Aspect_securityTradeGrossAmount
mgx:_Aspect_securityTradeGrossAmount rdf:type owl:NamedIndividual ,
                                              gist:Aspect ;
                                     <http://www.w3.org/2004/02/skos/core#definition> <https://w3id.org/moneygraph/o/ontology/> ,
                                                                                      "Share unit price multiplied by number of shares purchased or sold." .


###  https://w3id.org/moneygraph/ns/taxonomy/_Aspect_securityTradeInterestAmount
mgx:_Aspect_securityTradeInterestAmount rdf:type owl:NamedIndividual ,
                                                 gist:Aspect ;
                                        <http://www.w3.org/2004/02/skos/core#definition> "Accumulated bond (or other debt security) interest amount either paid or received at the time of the trade." ;
                                        <http://www.w3.org/2004/02/skos/core#prefLabel> "security trade interest amount" .


###  https://w3id.org/moneygraph/ns/taxonomy/_Aspect_securityTradeNetAmount
mgx:_Aspect_securityTradeNetAmount rdf:type owl:NamedIndividual ,
                                            gist:Aspect ;
                                   rdfs:seeAlso <https://w3id.org/moneygraph/o/ontology/> ;
                                   <http://www.w3.org/2004/02/skos/core#definition> "Share unit price multiplied by number of shares purchased or sold, plus/minus commission fees." .


###  https://w3id.org/moneygraph/ns/taxonomy/_Aspect_securityTradeTransactionCommission
mgx:_Aspect_securityTradeTransactionCommission rdf:type owl:NamedIndividual ,
                                                        gist:Aspect ;
                                               rdfs:isDefinedBy <https://w3id.org/moneygraph/o/ontology/> ;
                                               <http://www.w3.org/2004/02/skos/core#definition> "Fee assessed for security transactions such as buying, selling, or transferring." .


###  https://w3id.org/moneygraph/ns/taxonomy/_Aspect_yieldToMaturity
mgx:_Aspect_yieldToMaturity rdf:type owl:NamedIndividual ,
                                     gist:Aspect .


###  https://w3id.org/moneygraph/ns/taxonomy/_CADollar
mgx:_CADollar rdf:type owl:NamedIndividual ,
                       gist:CurrencyUnit ;
              <http://www.w3.org/2004/02/skos/core#definition> "Loonies and twonies and more." ;
              <http://www.w3.org/2004/02/skos/core#prefLabel> "Canadian Dollar" ;
              gist:unitSymbol "CAD" .


###  https://w3id.org/moneygraph/ns/taxonomy/_FinancialBusinessEventType_assetMerger
mgx:_FinancialBusinessEventType_assetMerger rdf:type owl:NamedIndividual ,
                                                     gist:FinancialBusinessEventType ;
                                            rdfs:isDefinedBy <https://w3id.org/moneygraph/o/ontology/> ;
                                            <http://www.w3.org/2004/02/skos/core#definition> "Asset mergers may result in shares of one asset being replaced by shares of another asset." .


###  https://w3id.org/moneygraph/ns/taxonomy/_FinancialBusinessEventType_debtPrincipalRepayment
mgx:_FinancialBusinessEventType_debtPrincipalRepayment rdf:type owl:NamedIndividual ,
                                                                gist:FinancialBusinessEventType ;
                                                       rdfs:isDefinedBy <https://w3id.org/moneygraph/o/ontology/> ;
                                                       <http://www.w3.org/2004/02/skos/core#definition> "Some or part of the principal of a debt is repaid." ;
                                                       <http://www.w3.org/2004/02/skos/core#example> "Repayment in full of a bond at maturity would be represented by this event type." .


###  https://w3id.org/moneygraph/ns/taxonomy/_FinancialBusinessEventType_deposit
mgx:_FinancialBusinessEventType_deposit rdf:type owl:NamedIndividual ,
                                                 gist:FinancialBusinessEventType ;
                                        rdfs:isDefinedBy <https://w3id.org/moneygraph/o/ontology/> ;
                                        <http://www.w3.org/2004/02/skos/core#definition> "Money is placed into an account." ;
                                        <http://www.w3.org/2004/02/skos/core#prefLabel> "deposit" .


###  https://w3id.org/moneygraph/ns/taxonomy/_FinancialBusinessEventType_dividendRemittance
mgx:_FinancialBusinessEventType_dividendRemittance rdf:type owl:NamedIndividual ,
                                                            gist:FinancialBusinessEventType ;
                                                   rdfs:isDefinedBy <https://w3id.org/moneygraph/o/ontology/> ;
                                                   <http://www.w3.org/2004/02/skos/core#definition> "The remittance of money from an asset dividend, e.g. a stock dividend." .


###  https://w3id.org/moneygraph/ns/taxonomy/_FinancialBusinessEventType_exchangeCurrency
mgx:_FinancialBusinessEventType_exchangeCurrency rdf:type owl:NamedIndividual ,
                                                          gist:FinancialBusinessEventType ;
                                                 rdfs:isDefinedBy <https://w3id.org/moneygraph/o/ontology/> ;
                                                 <http://www.w3.org/2004/02/skos/core#definition> "Changing US dollars into Canadian dollars, for example." .


###  https://w3id.org/moneygraph/ns/taxonomy/_FinancialBusinessEventType_interestRemittance
mgx:_FinancialBusinessEventType_interestRemittance rdf:type owl:NamedIndividual ,
                                                            gist:FinancialBusinessEventType ;
                                                   rdfs:isDefinedBy <https://w3id.org/moneygraph/o/ontology/> ;
                                                   <http://www.w3.org/2004/02/skos/core#definition> "The receipt of interest money from a loan or security." .


###  https://w3id.org/moneygraph/ns/taxonomy/_FinancialInstrument_cash
mgx:_FinancialInstrument_cash rdf:type owl:NamedIndividual ,
                                       gist:FinancialInstrument ;
                              <http://www.w3.org/2004/02/skos/core#prefLabel> "cash" .


###  https://w3id.org/moneygraph/ns/taxonomy/_MarketableSecurityIdentifierType_CUSIP
mgx:_MarketableSecurityIdentifierType_CUSIP rdf:type owl:NamedIndividual ,
                                                     mg:MarketableSecurityIdentifierType ;
                                            rdfs:seeAlso "https://en.wikipedia.org/wiki/CUSIP"^^xsd:anyURI ;
                                            <http://www.w3.org/2004/02/skos/core#definition> "A CUSIP (/ˈkjuːsɪp/) is a nine-character numeric or alphanumeric code (e.g. 037833100 for Apple) that uniquely identifies a North American financial security for the purposes of facilitating clearing and settlement of trades. (Wikipedia)" ;
                                            <http://www.w3.org/2004/02/skos/core#prefLabel> "Marketable Security ID Type: CUSIP" .


###  https://w3id.org/moneygraph/ns/taxonomy/_MarketableSecurityIdentifierType_qtBondId
mgx:_MarketableSecurityIdentifierType_qtBondId rdf:type owl:NamedIndividual ,
                                                        mg:MarketableSecurityIdentifierType ;
                                               <http://www.w3.org/2004/02/skos/core#definition> "ID used by Questrade to identify bonds." ;
                                               <http://www.w3.org/2004/02/skos/core#prefLabel> "Marketable Security ID Type: QT Bond ID" .


###  https://w3id.org/moneygraph/ns/taxonomy/_MarketableSecurityIdentifierType_tickerSymbol
mgx:_MarketableSecurityIdentifierType_tickerSymbol rdf:type owl:NamedIndividual ,
                                                            mg:MarketableSecurityIdentifierType ;
                                                   <http://www.w3.org/2004/02/skos/core#prefLabel> "Marketable Security ID Type : ticker symbol" .


###  https://w3id.org/moneygraph/ns/taxonomy/_MarketableSecurityType_bond
mgx:_MarketableSecurityType_bond rdf:type owl:NamedIndividual ,
                                          mg:MarketableSecurityType .


###  https://w3id.org/moneygraph/ns/taxonomy/_MarketableSecurityType_common_stock
mgx:_MarketableSecurityType_common_stock rdf:type owl:NamedIndividual ,
                                                  mg:MarketableSecurityType .


###  https://w3id.org/moneygraph/ns/taxonomy/_MarketableSecurityType_exchange_traded_fund
mgx:_MarketableSecurityType_exchange_traded_fund rdf:type owl:NamedIndividual ,
                                                          mg:MarketableSecurityType .


###  https://w3id.org/semanticarts/ns/ontology/gist/_one_day
gist:_one_day rdf:type owl:NamedIndividual .


###  https://w3id.org/semanticarts/ns/ontology/gist/_one_millisecond
gist:_one_millisecond rdf:type owl:NamedIndividual .


###  https://w3id.org/semanticarts/ns/ontology/gist/_one_minute
gist:_one_minute rdf:type owl:NamedIndividual .


#################################################################
#    General axioms
#################################################################

[ rdf:type owl:AllDifferent ;
  owl:distinctMembers ( mgx:_CADollar
                        gist:_USDollar
                        gist:_kelvin
                        gist:_kilogram
                        gist:_meter
                        gist:_millisecond
                        gist:_minute
                        gist:_mole
                        gist:_one_day
                        gist:_one_millisecond
                        gist:_one_minute
                        gist:_second
                      )
] .


###  Generated by the OWL API (version 4.5.26.2023-07-17T20:34:13Z) https://github.com/owlcs/owlapi
